Formula.v
@@ -16,23 +16,27 @@ Require Import UserTactics.
 (*rewrite to_list l*)
 Create HintDb list'.
 
-(*non-empty list*)
+(*non-empty list
 Inductive list' (A : Type) : Type :=
  | singleton : A -> list' A
  | cons' : A -> list' A -> list' A.
-
+*)
 
 Inductive formula : Set :=
   | atom (a : label) : formula
-  | arr (phi : list' formula) (t : formula) : formula.
-(*intersections are non-empty in the Coppo-Dezani type assingnment system*)
+  | arr (phi : list formula) (t : formula) : formula.
+(*intersections may be empty (omega) in the strict system*)
+
+Definition formula' := list formula.
+
 
 (*used to define rank, lists with at least two elements are assigned at least the value 1*)
-Definition rank_formula_aux' (f : formula -> nat) : list' formula -> nat :=
-  fix maxby_rec' (l: list' formula) :=
+Definition rank_formula_aux' (f : formula -> nat) : formula' -> nat :=
+  fix maxby_rec' (l: list formula) :=
     match l with
-    | (singleton x) => f x
-    | (cons' x xs) => Nat.max (maxby_rec' xs) (Nat.max (f x) 1)
+    | [] => 1
+    | [x] => f x
+    | (cons x xs) => Nat.max (maxby_rec' xs) (Nat.max (f x) 1)
     end.
 
 Fixpoint rank_formula (t : formula) : nat :=
@@ -41,53 +45,22 @@ Fixpoint rank_formula (t : formula) : nat :=
   | (arr phi s) => Nat.max (1 + rank_formula_aux' rank_formula phi) (rank_formula s)
   end.
 
-Definition rank_formula' (phi : list' formula) := rank_formula_aux' rank_formula phi.
+Definition rank_formula' (phi : formula') := rank_formula_aux' rank_formula phi.
 
-
-Fixpoint to_list (A : Type) (l : list' A) : list A :=
-  match l with
-  | (singleton a) => cons a nil
-  | (cons' a l) => cons a (to_list l)
-  end.
-
-Fixpoint to_list' (A : Type) (a : A) (l : list A) : list' A :=
-  match l with
-  | nil => singleton a
-  | (cons b l) => cons' a (to_list' b l)
-  end.
-
-Lemma to_list_inv : forall (A : Type) (a : A) (l : list A), to_list (to_list' a l) = a :: l.
-Proof.
-move => A a l.
-elim : l a; cbn; auto.
-intros; by f_equal.
-Qed.
-
-Coercion to_list : list' >-> list.
-
-Lemma to_list_cons' : forall (T : Type) (a : T) (l : list' T), 
-  to_list (cons' a l) = a :: to_list l.
-Proof. intros; reflexivity. Qed.
-
-(*Definition formula' : Set := list' formula.*)
-Notation formula' := (list' formula).
 
 Definition label_to_atom (a : label) : formula := atom a.
-Definition formula_to_singleton (s : formula) : formula' := singleton s.
+Definition formula_to_singleton (s : formula) : formula' := [s].
 
 (*embedding formulae into singleton intersections*)
 Coercion formula_to_singleton : formula >-> formula'.
 Coercion label_to_atom : label >-> formula. 
 
-Lemma forall_exists_in_formula' : forall (P : formula -> Prop) (phi : formula'), Forall P phi -> exists (s : formula), In s phi /\ P s.
+
+Lemma forall_exists_in_formula' : forall (P : formula -> Prop) (phi : formula'), phi <> [] -> Forall P phi -> exists (s : formula), In s phi /\ P s.
 Proof.
 move => P; case.
-move => s; inversion.
-exists s; split; auto.
-by constructor.
-move => s phi; inversion.
+done.
+move => s ? _. inversion.
 exists s; split; auto.
 by constructor.
 Qed.
-
-Hint Rewrite @to_list_inv @to_list_cons' : list'.
