MainResult.v
@@ -11,7 +11,7 @@ Import ListNotations.
 (*common header end*)
 
 Require Import Derivation.
-Require Import CD_Derivation.
+Require Import StrictDerivation.
 Require Import Encoding.
 Require Import Soundness.
 Require Import Completeness.
@@ -20,31 +20,32 @@ Require Import Completeness.
 given set "rs" of rewriting rules of shape ab -> cd,
 we have that 0..0 ->* 1..1 for some positive number of symbols
 iff
-triangle is inhabited in the environment (Γ_init ++ Γ_step rs) by a normal form N in the Coppo-Dezani type assignment system.
+triangle is inhabited in the environment (Γ_init ++ Γ_step rs) by a normal form N in the Coppo-Dezani-Venneri (cf. Strict Type Assignment [1]) type assignment system [2].
 *)
 Theorem correctness : forall (rs : list rule), 
   (exists (m : nat), rewrites_to rs (repeat 0 (1+m)) (repeat 1 (1+m))) <->
   (exists (N : term), normal_form N /\
-    cd_derivation (Γ_init ++ Γ_step rs) N (singleton (atom triangle))).
+    strict_derivation (Γ_init ++ Γ_step rs) N (atom triangle)).
 Proof.
 intro; split.
 
 move => [m]. move /completeness => [n [M [?]]].
-move /cd_derivation_completeness.
+move /strict_derivation_completeness.
 move /(_ (well_formed_Γ_all rs)).
 eauto.
 
 move => [N [?]].
-move /cd_derivation_soundness => [n]. 
+move /strict_derivation_soundness => [n]. 
 move /soundness.
 eauto.
 Qed.
 
 Print Assumptions correctness.
 
+
 (*show that all environment types are at most rank 2 and the goal type is at most rank 3 (actually rank 0)*)
 Lemma rank_bound : 
-  (rank_formula' (singleton (atom triangle)) <= 3) /\ 
+  (rank_formula' (atom triangle) <= 3) /\ 
   (forall (rs : list rule) (x : label) (phi : formula'), 
     In (x, phi) (Γ_init ++ Γ_step rs) -> rank_formula' phi <= 2).
 Proof.
@@ -53,3 +54,8 @@ cbn; do ? constructor.
 apply : rank_environment_bound; eassumption.
 Qed.
 
+(*
+Bibliography
+[1] van Bakel S. Strict Intersection Types for the Lambda Calculus. ACM Computing Surveys, 2011. 43(3). doi:10.1145/1922649.1922657.
+[2] M. Coppo, M. Dezani-Ciancaglini, and B. Venneri. Functional characters of solvable terms. Zeitschrift für Mathematische Logik und Grundlagen der Mathematik, 27:45–58, 1981.
+*)
