StrictDerivation.v
@@ -1,0 +1,143 @@
+(*common header begin*)
+Require Import Utf8.
+From Coq Require Import ssreflect ssrfun ssrbool.
+Set Implicit Arguments.
+Unset Strict Implicit.
+Unset Printing Implicit Defensive.
+Set Maximal Implicit Insertion.
+
+Require Import List.
+Import ListNotations.
+(*common header end*)
+
+Require Export Formula.
+Require Export Term.
+
+Require Import Omega.
+Require Import UserTactics.
+Require Import ListFacts.
+Require Import Derivation.
+
+(*Γ is well formed, if any term variable appears at most once*)
+Inductive well_formed_environment : environment -> Prop :=
+  | wfe_nil : well_formed_environment nil
+  | wfe_cons : forall (x : label) (phi : formula') (Γ: environment), 
+    Forall (fun '(y, _) => x <> y) Γ -> well_formed_environment Γ -> well_formed_environment ((x, phi ) :: Γ).
+
+(*M is well formed, if it contains no unbound De Bruijn indices*)
+Definition well_formed_term (M : term) : Prop := lc 0 M.
+
+(*van Bakel, Strict Intersection Types for the Lambda Calculus, p. 24, 5 The strict system*)
+Inductive strict_derivation : environment -> term -> formula -> Prop :=
+  | strict_elim_cap : forall (Γ: environment) (x : label) (phi: formula') (t : formula), 
+    well_formed_environment Γ -> 
+    In (x, phi) Γ -> In t phi -> strict_derivation Γ (free_var x) t
+  | strict_intro_arr : forall (Γ: environment) (M : term) (x : label) (phi : formula') (t : formula), 
+    well_formed_environment ((x, phi) :: Γ) -> well_formed_term M ->
+    strict_derivation ((x, phi) :: Γ) M t -> strict_derivation Γ (term_abs (bind x 0 M)) (arr phi t)
+  | strict_elim_arr : forall (Γ: environment) (M N : term) (phi : formula') (t : formula), 
+    well_formed_environment Γ -> well_formed_term M -> well_formed_term N ->
+    strict_derivation Γ M (arr phi t) -> strict_derivation_cap Γ N phi -> strict_derivation Γ (term_app M N) t
+with strict_derivation_cap : environment -> term -> formula' -> Prop :=
+  | strict_intro_cap : forall (Γ: environment) (M : term) (phi: formula'), 
+    well_formed_environment Γ -> well_formed_term M ->
+    Forall (strict_derivation Γ M) phi -> strict_derivation_cap Γ M phi.
+
+Lemma strict_derivation_completeness : forall (n : nat) (Γ: environment) (M : term) (t : formula), 
+  well_formed_environment Γ -> derivation n Γ M t -> strict_derivation Γ M t.
+Proof.
+elim /lt_wf_ind => n IH.
+intros; gimme derivation; inversion.
+
+apply : strict_elim_cap; eassumption.
+
+{(*abs*)
+match goal with [M' : term |- _] => rename M' into M end.
+have := exists_fresh M Γ; move => [x [? ?]].
+gimme where instantiate. 
+move /(_ x) => HD.
+move /derivation_lc : (HD) => ?.
+
+erewrite <- (bind_instantiate 0 (M:=M)); try eassumption.
+apply : strict_intro_arr; auto.
+by constructor.
+
+apply : IH; last eassumption; first omega.
+by constructor.
+}
+
+{(*app*)
+apply : strict_elim_arr; try trivial.
+
+apply : derivation_lc; eassumption.
+
+apply : (IH); last eassumption; first omega; auto.
+apply : strict_intro_cap; auto. 
+apply : Forall_impl; last eassumption.
+eauto.
+}
+Qed.
+
+
+Lemma strict_derivation_soundness : forall (Γ: environment) (M : term) (t : formula),
+   strict_derivation Γ M t -> exists (n : nat), derivation n Γ M t.
+Proof.
+intros *.
+have [m H_m] := exists_term_depth M.
+move : m Γ M t H_m.
+elim /lt_wf_ind.
+move => m IH; intros *.
+inversion; inversion.
+
+{(*case var*)
+exists 0; apply : ax; eassumption.
+}
+
+
+{(*case app*)
+match goal with [phi' : formula' |- _] => rename phi' into phi end.
+have : exists (n : nat), Forall (derivation n Γ N) phi.
+{(*show that N is uniformly typable wrt. depth*)
+gimme strict_derivation_cap; gimme strict_derivation => _.
+inversion.
+apply Forall_exists_monotone.
+
+intros; apply : derivation_relax_depth; [eassumption | omega].
+
+apply : Forall_impl; last eassumption.
+intros. apply : IH; try eassumption; omega.
+}
+
+gimme strict_derivation; move /IH.
+move /(_ _ _ ltac:(eassumption)). move /(_ ltac:(omega)) => [n1 ?] [n2 ?].
+exists (S (n1+n2)).
+apply : elim_arr.
+apply : derivation_relax_depth; eassumption + omega.
+apply : Forall_impl; last eassumption.
+intros; apply : derivation_relax_depth; eassumption + omega.
+done.
+}
+
+
+{(*case abs*)
+gimme strict_derivation.
+gimme term_depth.
+move /bind_depth => ?.
+move /IH. move /(_ _ _ ltac:(eassumption)). move /(_ ltac:(omega)) => [n' ?].
+exists (S n').
+gimme well_formed_environment; inversion.
+apply : fresh_abstraction_bind; auto.
+}
+Qed.
+
+(*typing environments may be arbitrarily permuted or extended as long as well-formedness is preserved*)
+Theorem strict_weakening : forall (Γ Γ': environment) (M: term) (t: formula), 
+  strict_derivation Γ M t -> well_formed_environment Γ' -> (forall (p : label * formula'), In p Γ -> In p Γ') -> strict_derivation Γ' M t.
+Proof.
+intros; gimme strict_derivation.
+move /strict_derivation_soundness => [n].
+move /weakening. move /(_ _ ltac:(eassumption)).
+move /strict_derivation_completeness. 
+auto.
+Qed.
+
